dispose

pulse/ulib/experimental/Steel.DisposableInvariant.fst
@@ -32,12 +32,15 @@ assume
 val gather_ghost (#a:Type) (#u:_)
                  (#[@@@framing_implicit]p0:perm)
                  (#[@@@framing_implicit]p1:perm)
-                 (#[@@@framing_implicit]x:erased a)
+                 (#[@@@framing_implicit]x0:erased a)
+                 (#[@@@framing_implicit]x1:erased a)
                  (r:ghostref a)
-  : SteelAtomicT unit u unobservable
-    (ghost_pts_to r p0 x `star`
-     ghost_pts_to r p1 x)
-    (fun _ -> ghost_pts_to r (sum_perm p0 p1) x)
+  : SteelAtomic unit u unobservable
+    (ghost_pts_to r p0 x0 `star`
+     ghost_pts_to r p1 x1)
+    (fun _ -> ghost_pts_to r (sum_perm p0 p1) x0)
+    (requires fun _ -> true)
+    (ensures fun _ _ _ -> x0 == x1)
 
 assume
 val write_ghost (#a:Type) (#u:_) (#x:erased a) (r:ghostref a) (v:erased a)
@@ -52,6 +55,7 @@ let conditional_inv (r:ghostref bool) (p:slprop) =
          ghost_pts_to r (half_perm full_perm) (hide b) `star`
          (if b then p else emp))
 
+[@@__reduce__]
 let ex_conditional_inv (r:ghostref bool) (p:slprop) =
     h_exists (conditional_inv r p)
 
@@ -93,11 +97,11 @@ let gather (#p:slprop) (#f0 #f1:perm) (#u:_) (i:inv p)
   : SteelAtomicT unit u unobservable
     (active f0 i `star` active f1 i)
     (fun _ -> active (sum_perm f0 f1) i)
-  = gather_ghost #_ #_ #(half_perm f0) #(half_perm f1) #(hide true) (gref i);
+  = gather_ghost #_ #_ #(half_perm f0) #(half_perm f1) (gref i);
     A.change_slprop
       (ghost_pts_to (gref i) (sum_perm (half_perm f0) (half_perm f1)) (hide true))
       (ghost_pts_to (gref i) (half_perm (sum_perm f0 f1)) (hide true))
-      (fun _ -> assert (FStar.Real.two == 2.0R))
+      (fun _ -> assert (FStar.Real.two == 2.0R); assert (sum_perm (half_perm f0) (half_perm f1) == (half_perm (sum_perm f0 f1))))
 
 assume
 val drop (#u:_) (p:slprop)
@@ -105,23 +109,32 @@ val drop (#u:_) (p:slprop)
 
 let iinv (#p:_) (i:inv p) : Steel.Memory.inv (ex_conditional_inv (gref i) p) = name i
 
-let dispose' (#p:slprop) (#u:_) (i:inv p{not (name i `Set.mem` u)})
-  : SteelAtomicT unit u unobservable
-    (active full_perm i)
-    (fun _ -> p)
-  = let dispose_aux (r:ghostref bool) (_:unit)
-     : SteelAtomicT unit (set_add (name i) u)  unobservable
+let dispose_aux #u #p (r:ghostref bool) (i:inv p) (_:unit)
+  : SteelAtomicT unit (set_add (name i) u)  unobservable
        (ex_conditional_inv r p `star`
         ghost_pts_to r (half_perm full_perm) true)
        (fun _ ->
         ex_conditional_inv r p `star`
         p)
-     = admit_atomic #unit #u ()
-    in
-    A.with_invariant #unit #(ghost_pts_to (gref i) (half_perm full_perm) true)
+  = let b = A.witness_h_exists #_ #_ #(conditional_inv r p) () in
+    gather_ghost #_ #_ #(half_perm full_perm) #(half_perm full_perm) #true #(hide (reveal b)) r;
+    A.change_slprop (if b then p else emp) p (fun _ -> ());
+    A.change_slprop (ghost_pts_to r (sum_perm (half_perm full_perm) (half_perm full_perm)) true)
+                    (ghost_pts_to r full_perm true)
+                    (fun _ -> ());
+    write_ghost r false;
+    split_ghost r;
+    A.intro_h_exists false (conditional_inv r p);
+    drop (ghost_pts_to r (half_perm full_perm) false)
+
+let dispose (#p:slprop) (#u:_) (i:inv p{not (name i `Set.mem` u)})
+  : SteelAtomicT unit u unobservable
+    (active full_perm i)
+    (fun _ -> p)
+  = A.with_invariant #unit #(ghost_pts_to (gref i) (half_perm full_perm) true)
                            #(fun _ -> p)
                            #u
                            #unobservable
                            #(ex_conditional_inv (gref i) p)
                            (iinv i)
-                           (dispose_aux (gref i))
+                           (dispose_aux #u #p (gref i) i)
